compiler/src/compiler/Simulation.v
@@ -5,14 +5,16 @@ Our simulations, however, talk about all executions at once and about single sta
 "All states in the low-level outcome set have a corresponding state in the high-level outcome set".
 *)
 
+(* "related" takes a "done" flag which tells whether we're comparing the states before or
+   after executing the code *)
 Definition simulation{State1 State2: Type}
            (exec1: State1 -> (State1 -> Prop) -> Prop)
            (exec2: State2 -> (State2 -> Prop) -> Prop)
-           (related: State1 -> State2 -> Prop): Prop :=
+           (related: bool -> State1 -> State2 -> Prop): Prop :=
   forall s1 s2 post1,
-    related s1 s2 ->
+    related false s1 s2 ->
     exec1 s1 post1 ->
-    exec2 s2 (fun s2' => exists s1', related s1' s2' /\ post1 s1').
+    exec2 s2 (fun s2' => exists s1', related true s1' s2' /\ post1 s1').
 
 Definition compile_inv{State1 State2: Type}
            (related: State1 -> State2 -> Prop)(inv: State1 -> Prop): State2 -> Prop :=
@@ -27,11 +29,11 @@ Definition is_inv{State: Type}(exec: State -> (State -> Prop) -> Prop)(inv: Stat
 Lemma compile_inv_is_inv{State1 State2: Type}
       (exec1: State1 -> (State1 -> Prop) -> Prop)
       (exec2: State2 -> (State2 -> Prop) -> Prop)
-      (related: State1 -> State2 -> Prop)
+      (related: bool -> State1 -> State2 -> Prop)
       (Sim: simulation exec1 exec2 related)
       (inv1: State1 -> Prop)
       (inv1_is_inv: forall s1, inv1 s1 -> exec1 s1 inv1):
-  forall s2, compile_inv related inv1 s2 -> exec2 s2 (compile_inv related inv1).
+  forall s2, compile_inv (related false) inv1 s2 -> exec2 s2 (compile_inv (related true) inv1).
 Proof.
   unfold compile_inv, simulation in *.
   intros s2 (s1 & R & I1).
@@ -41,9 +43,9 @@ Proof.
 Qed.
 
 Definition compose_relation{State1 State2 State3: Type}
-           (R12: State1 -> State2 -> Prop)(R23: State2 -> State3 -> Prop):
-  State1 -> State3 -> Prop :=
-  fun s1 s3 => exists s2, R12 s1 s2 /\ R23 s2 s3.
+           (R12: bool -> State1 -> State2 -> Prop)(R23: bool -> State2 -> State3 -> Prop):
+  bool -> State1 -> State3 -> Prop :=
+  fun done s1 s3 => exists s2, R12 done s1 s2 /\ R23 done s2 s3.
 
 Definition weakening{State: Type}(exec: State -> (State -> Prop) -> Prop): Prop :=
   forall (post1 post2: State -> Prop),
@@ -55,8 +57,8 @@ Lemma compose_simulation{State1 State2 State3: Type}
       (exec2: State2 -> (State2 -> Prop) -> Prop)
       (exec3: State3 -> (State3 -> Prop) -> Prop)
       (W3: weakening exec3)
-      (R12: State1 -> State2 -> Prop)
-      (R23: State2 -> State3 -> Prop)
+      (R12: bool -> State1 -> State2 -> Prop)
+      (R23: bool -> State2 -> State3 -> Prop)
       (S12: simulation exec1 exec2 R12)
       (S23: simulation exec2 exec3 R23):
   simulation exec1 exec3 (compose_relation R12 R23).
@@ -79,8 +81,8 @@ Lemma compose_sim{State1 State2 State3: Type}
       {exec1: State1 -> (State1 -> Prop) -> Prop}
       {exec2: State2 -> (State2 -> Prop) -> Prop}
       {exec3: State3 -> (State3 -> Prop) -> Prop}
-      {R12: State1 -> State2 -> Prop}
-      {R23: State2 -> State3 -> Prop}
+      {R12: bool -> State1 -> State2 -> Prop}
+      {R23: bool -> State2 -> State3 -> Prop}
       (S12: simulation exec1 exec2 R12)
       (S23: simulation exec2 exec3 R23):
   simulation exec1 exec3 (compose_relation R12 R23).
